### CLSCor Data Model (DRAFT) ###

@prefix crm: <http://www.cidoc-crm.org/cidoc-crm/> .
@prefix crmcls: <https://clscor.io/ontologies/CRMcls/> .
@prefix crmdig: <http://www.ics.forth.gr/isl/CRMdig/> .
@prefix dce: <http://purl.org/dc/elements/1.1/> .
@prefix frbroo: <http://iflastandards.info/ns/fr/frbr/frbroo/> .
@prefix lrm: <http://iflastandards.info/ns/lrm/lrmoo/> .
@prefix owl: <http://www.w3.org/2002/07/owl#> .
@prefix pem: <http://parthenos.d4science.org/CRMext/CRMpe.rdfs> .
@prefix rdf: <http://www.w3.org/1999/02/22-rdf-syntax-ns#> .
@prefix rdfs: <http://www.w3.org/2000/01/rdf-schema#> .

#################################################################
# Ontology
#################################################################

<https://clscor.io/ontologies/CRMcls> a owl:Ontology ;
    rdfs:label "CRM CLS" ;
    rdfs:comment "Ontology for describing corpora relevant to Computational Literary Studies. This ontology was developed in the context of the CLS INFRA Project."@en ;
    owl:versionInfo "v.0.1.0" ;
    dce:creator "Vera Maria Charvat", "Ingo Börner", "Matej Durco", "Lukas Plank" ;
    dce:contributor "George Bruseker", "Michal Mrugalski", "Carolin Odebrecht", "Stefan Resch", "Salvador Ros" .

#################################################################
# Introduced classes
#################################################################

crmcls:X1_Corpus a owl:Class, rdfs:Class ;
    rdfs:label "Korpus"@de ,
        "Corpus"@en ;
    rdfs:comment "This class stands for a corpus or text corpus. A corpus is a set or dataset, consisting of one or more corpus documents."@en ;
    rdfs:subClassOf lrm:F3_Manifestation ,
        crmdig:D1_Digital_Object ;
    rdfs:isDefinedBy <https://clscor.io/ontologies/CRMcls> .

crmcls:X2_Corpus_Document a owl:Class, rdfs:Class ;
    rdfs:label "Korpus-Dokument"@de ,
        "Corpus Document"@en ;
    rdfs:comment "This class stands for a corpus document, a container for different representations / expressions of a text. A corpus document is a single entity in a corpus."@en ;
    rdfs:subClassOf lrm:F3_Manifestation ,
        crmdig:D1_Digital_Object ;
    rdfs:isDefinedBy <https://clscor.io/ontologies/CRMcls> .
	
crmcls:X3_Feature a owl:Class, rdfs:Class ;
    rdfs:label "Feature"@de ,
        "Feature"@en ;
    rdfs:comment "This class stands for a feature, which allows to capture individual (atomic) aspects exhibited by a document or a set of documents. A feature is the output produced by a method (e.g., method 'Part of speech tagging' produces the feature 'part of speech tags')"@en ;
    rdfs:subClassOf crm:E73_Information_Object , crm:E58_Measurement_Unit ;
    rdfs:isDefinedBy <https://clscor.io/ontologies/CRMcls> .

crmcls:X4_Project a owl:Class, rdfs:Class ;
    rdfs:label "(Forschungs-)Projekt"@de ,
        "(Research) Project"@en ;
    rdfs:comment "This class stands for a project, which is 'an individual or collaborative enterprise that is carefully planned to achieve a particular aim' (cited from the Oxford dictionary)."@en ;
    rdfs:subClassOf crm:E7_Activity ;
    rdfs:isDefinedBy <https://clscor.io/ontologies/CRMcls> .

crmcls:X5_Research_Activity a owl:Class, rdfs:Class ;
    rdfs:label "Forschungsaktivität"@de ,
        "Research Activity"@en ;
    rdfs:comment "This class stands for a research activity, which describes 'the systematic search for new findings and their documentation and publication' (translated from the German Wikipedia article: https://de.wikipedia.org/wiki/Forschung) ."@en ;
    rdfs:subClassOf crm:E7_Activity ;
    rdfs:isDefinedBy <https://clscor.io/ontologies/CRMcls> .

crmcls:X6_Method a owl:Class, rdfs:Class ;
    rdfs:label "Methode"@de ,
        "Method"@en ;
    rdfs:comment "This class stands for a method, which (in the CLSCor context) is a particular procedure for approaching/completing a task."@en ;
    rdfs:subClassOf crm:E29_Design_or_Procedure ;
    rdfs:isDefinedBy <https://clscor.io/ontologies/CRMcls> .

crmcls:X7_Format a owl:Class, rdfs:Class ;
    rdfs:label "Format"@de ,
        "Format"@en ;
    rdfs:comment "This class stands for a format, which (in the CLSCor context) is a file format."@en ;
    owl:equivalentClass pem:PE43_Encoding_Type ;
    rdfs:isDefinedBy <https://clscor.io/ontologies/CRMcls> .

crmcls:X8_Schema a owl:Class, rdfs:Class ;
    rdfs:label "Schema"@de ,
        "Schema"@en ;
    rdfs:comment "This class stands for a schema, which is a document formally expressing allowed structures a format may follow."@en ;
    owl:equivalentClass pem:PE38_Schema ;
    rdfs:isDefinedBy <https://clscor.io/ontologies/CRMcls> .

crmcls:X9_Corpus_Description a owl:Class, rdfs:Class ;
    rdfs:label "Aktivität der Korpusbeschreibung"@de ,
        "Corpus Description Activity"@en ;
    rdfs:comment """This class stands for a corpus description activity/event, which describes the activity of collectiong metadata about 
        a corpus by using E13_Attribute_Assignment's. These individual attribute assignments are grouped under a 
        crmcls:X9_Corpus_Description event, which allows to efficiently capture, who, when and based on which sources the information 
        about the corpus was produced."""@en ;
    rdfs:subClassOf crm:E83_Type_Creation ;
    rdfs:isDefinedBy <https://clscor.io/ontologies/CRMcls> .

crmcls:X10_Encoding_Pattern a owl:Class, rdfs:Class ;
    rdfs:label "Encoding Vorlage"@de ,
        "Encoding Pattern"@en ;
    rdfs:comment "This class stands for an encoding pattern, which describes the pattern an encoding follows."@en ;
    rdfs:subClassOf crm:E90_Symbolic_Object ;
    rdfs:isDefinedBy <https://clscor.io/ontologies/CRMcls> .

crmcls:X11_Prototypical_Document a owl:Class, rdfs:Class ;
    rdfs:label "Prototypisches Dokument"@de ,
        "Prototypical Document"@en ;
    rdfs:comment """This class stands for a prototypical document, which serves as a surrogate entity for a single document inside a 
        corpus, to deal with the problem of uncertainties when providing information on document level. This allows to distinguish if 
        properties are assigned to a corpus as a whole (e.g., number of documents in corpus, number of words in corpus, corpusTimespan, 
        corpusType) or to the documents it consists of (e.g., language, format, feature, license, etc.) without necessarily inspecting 
        all of them."""@en ;
    rdfs:subClassOf crm:E55_Type ;
    rdfs:isDefinedBy <https://clscor.io/ontologies/CRMcls> .
	
crmcls:X12_Tool a owl:Class, rdfs:Class ;
	rdfs:label "Tool"@de ,
        "Tool"@en ;
    rdfs:comment """This class stands for a tool [...definition to be added...]"""@en ;
    rdfs:isDefinedBy <https://clscor.io/ontologies/CRMcls> .
	
crmcls:X13_Tool_Description a owl:Class, rdfs:Class ;
    rdfs:label "Aktivität der Toolbeschreibung"@de ,
        "Tool Description Activity"@en ;
    rdfs:comment "This class stands for a tool description activity/event, which describes the activity of collectiong metadata about a tool by using E13_Attribute_Assignment's. These individual attribute assignments are grouped under a crmcls:X13_Tool_Description event, which allows to efficiently capture, who, when and based on which sources the information about the tool was produced."@en ;
    rdfs:subClassOf crm:E83_Type_Creation ;
    rdfs:isDefinedBy <https://clscor.io/ontologies/CRMcls> .

#################################################################
# Introduced properties
#################################################################

crmcls:Y1_exhibits_feature a owl:ObjectProperty, rdf:Property ;
    rdfs:label "enthält Feature"@de,
        "exhibits feature"@en ;
    rdfs:comment "states that a corpus document or prototypical document exhibits a feature"@en ;
    rdfs:domain crmcls:X2_Corpus_Document, crmcls:X11_Prototypical_Document ;
    rdfs:range crmcls:X3_Feature ;
    owl:inverseOf crmcls:Y1i_feature_is_exhibited_by ;
    rdfs:isDefinedBy <https://clscor.io/ontologies/CRMcls> .

crmcls:Y1i_feature_is_exhibited_by a owl:ObjectProperty, rdf:Property ;
    rdfs:label "Feature ist enthalten in"@de,
        "feature is exhibited by"@en ;
    rdfs:comment "states a feature which is exhibited by a corpus document or prototypical document"@en ;
    rdfs:domain crmcls:X3_Feature ;
    rdfs:range crmcls:X2_Corpus_Document, crmcls:X11_Prototypical_Document ;
    owl:inverseOf crmcls:Y1_exhibits_feature ;
    rdfs:isDefinedBy <https://clscor.io/ontologies/CRMcls> .

crmcls:Y2_has_format a owl:ObjectProperty, rdf:Property ;
    rdfs:label "hat Format"@de,
        "has format"@en ;
    rdfs:comment "states that a corpus document or prototypical document is available in a format"@en ;
    rdfs:domain crmcls:X2_Corpus_Document, crmcls:X11_Prototypical_Document ;
    rdfs:range pem:PE43_Encoding_Type ;
    owl:inverseOf crmcls:Y2i_is_format_of ;
    rdfs:isDefinedBy <https://clscor.io/ontologies/CRMcls> .

crmcls:Y2i_is_format_of a owl:ObjectProperty, rdf:Property ;
    rdfs:label "ist Format von"@de,
        "is format of"@en ;
    rdfs:comment "states the format a corpus document or prototypical document is available in"@en ;
    rdfs:domain pem:PE43_Encoding_Type ;
    rdfs:range crmcls:X2_Corpus_Document, crmcls:X11_Prototypical_Document ;
    owl:inverseOf crmcls:Y2_has_format ;
    rdfs:isDefinedBy <https://clscor.io/ontologies/CRMcls> .

crmcls:Y3_adheres_to_schema a owl:ObjectProperty, rdf:Property ;
    rdfs:label "folgt Schema"@de,
        "adheres to schema"@en ;
    rdfs:comment "states that a corpus document or prototypical document adheres to a schema"@en ;
    rdfs:domain crmcls:X2_Corpus_Document, crmcls:X11_Prototypical_Document ;
    rdfs:range pem:PE38_Schema ;
    owl:inverseOf crmcls:Y3i_is_schema_of ;
    rdfs:isDefinedBy <https://clscor.io/ontologies/CRMcls> .

crmcls:Y3i_is_schema_of a owl:ObjectProperty, rdf:Property ;
    rdfs:label "ist Schema von"@de,
        "is schema of"@en ;
    rdfs:comment "states a schema to which a corpus document or prototypical document adheres to"@en ;
    rdfs:domain pem:PE38_Schema ;
    rdfs:range crmcls:X2_Corpus_Document, crmcls:X11_Prototypical_Document ;
    owl:inverseOf crmcls:Y3_adheres_to_schema ;
    rdfs:isDefinedBy <https://clscor.io/ontologies/CRMcls> .

crmcls:Y4_has_subcorpus a owl:ObjectProperty, rdf:Property ;
    rdfs:label "hat als Subkorpus"@de,
        "has subcorpus"@en ;
    rdfs:comment "associates a corpus with its subcorpus"@en ;
    rdfs:domain crmcls:X1_Corpus ;
    rdfs:range crmcls:X1_Corpus ;
    rdfs:subPropertyOf crm:P148_has_component ;
    owl:inverseOf crmcls:Y4i_is_subcorpus_of ;
    rdfs:isDefinedBy <https://clscor.io/ontologies/CRMcls> .

crmcls:Y4i_is_subcorpus_of a owl:ObjectProperty, rdf:Property ;
    rdfs:label "ist Subkorpus von"@de,
        "is subcorpus of"@en ;
    rdfs:comment "associates a subcorpus with its super corpus"@en ;
    rdfs:domain crmcls:X1_Corpus ;
    rdfs:range crmcls:X1_Corpus ;
    rdfs:subPropertyOf crm:P148i_is_component_of ;
    owl:inverseOf crmcls:Y4_has_subcorpus ;
    rdfs:isDefinedBy <https://clscor.io/ontologies/CRMcls> .

crmcls:Y5_encodes a owl:ObjectProperty, rdf:Property ;
    rdfs:label "enkodiert"@de,
        "encodes"@en ;
    rdfs:comment "states that an encoding pattern encodes a feature"@en ;
    rdfs:domain crmcls:X10_Encoding_Pattern ;
    rdfs:range crmcls:X3_Feature ;
    owl:inverseOf crmcls:Y5i_is_encoded_by ;
    rdfs:isDefinedBy <https://clscor.io/ontologies/CRMcls> .

crmcls:Y5i_is_encoded_by a owl:ObjectProperty, rdf:Property ;
    rdfs:label "wird kodiert durch"@de,
        "is encoded by"@en ;
    rdfs:comment "states that a feature is encoded following an encoding pattern"@en ;
    rdfs:domain crmcls:X3_Feature ;
    rdfs:range crmcls:X10_Encoding_Pattern ;
    owl:inverseOf crmcls:Y5_encodes ;
    rdfs:isDefinedBy <https://clscor.io/ontologies/CRMcls> .

crmcls:Y6_defines a owl:ObjectProperty, rdf:Property ;
    rdfs:label "definiert"@de,
        "defines"@en ;
    rdfs:comment "states that a procedure defines an encoding pattern."@en ;
    rdfs:domain crmcls:E29_Design_or_Procedure ;
    rdfs:range crmcls:X10_Encoding_Pattern ;
    owl:inverseOf crmcls:Y6i_is_defined_by ;
    rdfs:isDefinedBy <https://clscor.io/ontologies/CRMcls> .

crmcls:Y6i_is_defined_by a owl:ObjectProperty, rdf:Property ;
    rdfs:label "wird definiert durch"@de,
        "is defined by"@en ;
    rdfs:comment "states that an encoding pattern is defined by a procedure"@en ;
    rdfs:domain crmcls:X10_Encoding_Pattern ;
    rdfs:range crmcls:E29_Design_or_Procedure ;
    owl:inverseOf crmcls:Y6_defines ;
    rdfs:isDefinedBy <https://clscor.io/ontologies/CRMcls> .

crmcls:Y7_uses a owl:ObjectProperty, rdf:Property ;
    rdfs:label "verwendet"@de,
        "uses"@en ;
    rdfs:comment "[to be added]"@en ;
    rdfs:domain crmcls:X5_Research_Activity ,
		crmcls:X12_Tool ;
    rdfs:range crmcls:X12_Tool ;
    owl:inverseOf crmcls:Y7i_is_used_by ;
    rdfs:isDefinedBy <https://clscor.io/ontologies/CRMcls> .
	
crmcls:Y7i_is_used_by a owl:ObjectProperty, rdf:Property ;
    rdfs:label "wird verwendet von"@de,
        "is used by"@en ;
    rdfs:comment "[to be added]"@en ;
    rdfs:domain crmcls:X12_Tool ;
    rdfs:range crmcls:X5_Research_Activity ,
		crmcls:X12_Tool	;
    owl:inverseOf crmcls:Y7_uses ;
    rdfs:isDefinedBy <https://clscor.io/ontologies/CRMcls> .	
	
crmcls:Y8_implements a owl:ObjectProperty, rdf:Property ;
    rdfs:label "implementiert"@de,
        "implements"@en ;
    rdfs:comment "[to be added]"@en ;
    rdfs:domain crmcls:X12_Tool ;
    rdfs:range crmcls:X6_Method ;
    owl:inverseOf crmcls:Y8i_is_implemented_by ;
    rdfs:isDefinedBy <https://clscor.io/ontologies/CRMcls> .

crmcls:Y8i_is_implemented_by a owl:ObjectProperty, rdf:Property ;
    rdfs:label "wird implementiert durch"@de,
        "is implemented by"@en ;
    rdfs:comment "[to be added]"@en ;
    rdfs:domain crmcls:X6_Method ;
    rdfs:range crmcls:X12_Tool ;
    owl:inverseOf crmcls:Y8_implements ;
    rdfs:isDefinedBy <https://clscor.io/ontologies/CRMcls> .

crmcls:Y9_expects_input a owl:ObjectProperty, rdf:Property ;
    rdfs:label "erwartet Input"@de,
        "expects input"@en ;
    rdfs:comment "[to be added]"@en ;
    rdfs:domain crmcls:X6_Method ,
		crmcls:X12_Tool ;
    rdfs:range crmcls:X3_Feature ,
		crmcls:X7_Format ,
		crmcls:X8_Schema ;
    owl:inverseOf crmcls:Y9i_input_is_expected_by ;
    rdfs:isDefinedBy <https://clscor.io/ontologies/CRMcls> .

crmcls:Y9i_input_is_expected_by a owl:ObjectProperty, rdf:Property ;
    rdfs:label "Input wird erwartet von"@de,
        "input is expected by"@en ;
    rdfs:comment "[to be added]"@en ;
    rdfs:domain crmcls:X3_Feature ,
		crmcls:X7_Format ,
		crmcls:X8_Schema ;
    rdfs:range crmcls:X6_Method ,
		crmcls:X12_Tool ;
    owl:inverseOf crmcls:Y9_expects_input ;
    rdfs:isDefinedBy <https://clscor.io/ontologies/CRMcls> .
	
crmcls:Y10_generates_output a owl:ObjectProperty, rdf:Property ;
    rdfs:label "generiert Output"@de,
        "generates output"@en ;
    rdfs:comment "[to be added]"@en ;
    rdfs:domain crmcls:X6_Method ,
		crmcls:X12_Tool ;
    rdfs:range crmcls:X3_Feature ,
		crmcls:X7_Format ,
		crmcls:X8_Schema ;
    owl:inverseOf crmcls:Y10i_output_is_generated_by ;
    rdfs:isDefinedBy <https://clscor.io/ontologies/CRMcls> .

crmcls:Y10i_output_is_generated_by a owl:ObjectProperty, rdf:Property ;
    rdfs:label "Output wird generiert von"@de,
        "output is generated by"@en ;
    rdfs:comment "[to be added]"@en ;
    rdfs:domain crmcls:X3_Feature ,
		crmcls:X7_Format ,
		crmcls:X8_Schema ;
    rdfs:range crmcls:X6_Method ,
		crmcls:X12_Tool ;
    owl:inverseOf crmcls:Y10_generates_output ;
    rdfs:isDefinedBy <https://clscor.io/ontologies/CRMcls> .
	
